\documentclass[9pt]{beamer}
\include{config}

\usepackage{amssymb}
\usepackage{textcomp}

\definecolor{usccardinal}{rgb}{0.6, 0.0, 0.0}
\definecolor{bostonuniversityred}{rgb}{0.8, 0.0, 0.0}

\newcommand{\half}{\frac{1}{2}}
\newcommand{\dxdt}{\mathrm{d}x\mathrm{d}t}
\newcommand{\diff}{\mathrm{d}}
\newcommand{\iunit}{\mathrm{i}}
\newcommand{\e}[1]{\mathrm{e}^{#1}}
\newcommand{\expi}[1]{\mathrm{e}^{\mathrm{i}#1}}
\newcommand{\C}{\mathbb{C}}
\renewcommand{\L}{\mathcal{L}}
\newcommand{\I}{\mathcal{I}}
\newcommand{\partderi}[2]{\frac{\partial#1}{\partial#2}}

\newcommand{\red}{\color{red}}
\newcommand{\bur}{\color{bostonuniversityred}}
\newcommand{\blue}{\color{blue}}
\newcommand{\obs}{^\text{obs}}
\renewcommand{\cal}{^\text{cal}}
\newcommand{\comp}{^\text{comp}}
\newcommand{\true}{^\text{true}}
\newcommand{\bas}{_\text{bas}}
\newcommand{\mon}{_\text{mon}}

% \graphicspath{{Fig/}}

\AtBeginSection[]{
  \begin{frame}
    \tableofcontents[currentsection,currentsubsection]
  \end{frame}
}

%--------------------------------------------------------------------------------------
% \titlegraphic{\includegraphics[scale=0.5]{Fig/logo.pdf}\;\;\;\includegraphics[scale=0.2]{Fig/logo-ISTerre.png}}
\title{Fr\'echet derivatives under various parameterizations \\ using chain rule}
\subtitle{for LEGO module m\_parameterization.f90}
\author{joeyartech\\
\scriptsize{joeywzhou1986@gmail.com}}
\institute{The University of Texas at Dallas}
\date{10/18/2019}
%--------------------------------------------------------------------------------------


\begin{document}
%\small

\maketitle \clearpage

% \frame{
% \frametitle{Outline}
% \small{
% \tableofcontents[section,subsectionstyle=hide/show/show] }}

\begin{frame}\frametitle{Overview}

  \begin{block}{Physical meaning of symbols uniformly used in this code:}
  \begin{tabular}{ll}
    vp                   & P-wave velocity \\
    vs                   & S-wave velocity \\
    sp =1/vp             & P-wave slowness \\
    sps=vs/vp            & inv Vp-Vs ratio \\
    ip =vp*rho           & P-wave (acoustic) impedance \\
    rho                  & density \\
    kpa=rho*vp\^{}2         & bulk modulus \\
    lda=rho*(vp\^{}2-2vs\^{}2) & 1st Lam\'e parameter \\
    mu =rho*vs\^{}2         & 2nd Lam\'e parameter, shear modulus
  \end{tabular}
  \end{block}
  
\end{frame}

\begin{frame}\frametitle{Overview}
  
  \begin{block}{Considered parameterizations}
  \begin{tabular}{lll}
    \hline
    SITUATION    & PARAMETERIZATION & ALLOWED PARAMETERS \\
    \hline
    WaveEquation & moduli-density   & kpa (or lda mu) rho \\
    I/O models   & velocities-density & vp vs rho \\
    seismic      & velocities-impedance & vp vs ip \\
    tomography   & slowness-density     & sp sps rho \\
    optimization & can be any of above \\
    \hline
  \end{tabular} 
  \end{block} 

  \begin{block}{Source-Destination trilogy:}
    \centering \framebox{model m $\xrightarrow{FWD}$ WaveEq lm $\xrightarrow{PARAMETERIZATION}$ optim x,g $\xrightarrow{FWD}$ model m}
    
    \begin{itemize}
      \item model m $\rightarrow$ WaveEq lm depending on field.
      \item WaveEq produces gkpa (or glda, gmu) and grho under moduli-density parameterization.
      \item then m\_parameterization.f90 converts them to another parameterization for optim x,g, which can be any of parameterization
    \end{itemize}
  \end{block}
  
\end{frame}

\begin{frame}\frametitle{Overview}
  
  \begin{block}{ACTIVE versus PASSIVE}
  \begin{itemize}
    \item Active parameters will be converted to optim x via feature scaling (e.g. (par-par\_min)/(par\_max-par\_min)),
          and will be updated by optimization methods.
    \begin{itemize}
      \item Mono-parameter inversion: 1 active parameter.
      \item Multi-parameter inversion: $>1$ active parameters.
      \begin{itemize}
         \item Scaling in m\_linesearch.f90 depends only on the 1st active parameters (no matter of it's velocity or not).
         \item Output of inversion results has same sequence of active parameters listed in setup.in
      \end{itemize}
    \end{itemize}

    \item Passive parameters will NOT be converted to optim x, and will NOT be updated by optimization methods.
    \item However, they may still be updated according to user-specified empirical law (e.g. Gardner), which serves as hard constraints between parameters.
      \begin{itemize}
        \item User has to modified the code where necessary to insert such a law as symbolic computation is not straightforward in fortran
        \item Such a law may change the optim g for active parameters.
      \end{itemize}
      
  \end{itemize}
  \end{block}    

\end{frame}

\section{velocities-density}

\begin{frame}\frametitle{PARAMETERIZATION velocities-density}
\framesubtitle{isotropic ACoustic}
  
  \begin{minipage}{0.5\linewidth}
    \[\left\{ \begin{array}{l}
      \kappa = \rho V_P^2 \\
      \rho_0 = \rho 
    \end{array} \right.\]
    
    \begin{eqnarray}
      \nabla_{V_P} &=& \nabla_{\kappa} \partderi{\kappa}{V_P} + \nabla_{\rho_0} \partderi{\rho_0}{V_P} \nonumber\\
                   &=& \nabla_{\kappa} 2\rho V_P \nonumber\\
      \nabla_{\rho} &=& \nabla_{\kappa} \partderi{\kappa}{\rho} + \nabla_{\rho_0} \partderi{\rho_0}{\rho} \nonumber\\
		    &=& \nabla_{\kappa} V_P^2 + \nabla_{\rho_0} \nonumber
    \end{eqnarray}

  \end{minipage} \vline
  \begin{minipage}{0.45\linewidth}
    \[\left\{ \begin{array}{l}
      V_P  = \sqrt{\frac{\kappa}{\rho_0}} \\
      \rho = \rho_0
    \end{array} \right.\]
    
    \begin{eqnarray}
      \nabla_{\kappa} &=& \nabla_{V_P} \partderi{V_P}{\kappa} + \nabla_{\rho} \partderi{\rho}{\kappa} \nonumber\\
                      &=& \nabla_{V_P} \frac{1}{2\rho_0}\sqrt{\frac{\rho_0}{\kappa}} \nonumber\\
                      &=& \nabla_{V_P} 0.5\rho_0^{-0.5}\kappa^{-0.5} \nonumber\\
      \nabla_{\rho_0} &=& \nabla_{V_P} \partderi{V_P}{\rho_0} + \nabla_{\rho} \partderi{\rho}{\rho_0} \nonumber\\
                      &=& \nabla_{V_P} \left(-\frac{\kappa}{2\rho_0^2}\sqrt{\frac{\rho_0}{\kappa}}\right) + \nabla_{\rho} \nonumber\\
                      &=& \nabla_{V_P} \left(-0.5\rho_0^{-1.5}\kappa^{0.5}\right) + \nabla_{\rho} \nonumber
    \end{eqnarray}
  \end{minipage}

\end{frame}

\begin{frame}\frametitle{PARAMETERIZATION velocities-density + PASSIVE gardner}
\framesubtitle{isotropic ACoustic}

  \begin{center}
    \framebox{$\rho = a V_P ^{b}$}
  \end{center}

  \begin{minipage}{0.5\linewidth}
    \[\left\{ \begin{array}{l}
      \kappa = \rho V_P^2 = a V_P^{b+2} \\
      \rho_0 = \rho = a V_P ^{b}
    \end{array} \right.\]
    
    \begin{eqnarray}
      \nabla_{V_P} &=& \nabla_{\kappa} \partderi{\kappa}{V_P} + \nabla_{\rho_0} \partderi{\rho_0}{V_P} \nonumber\\
                   &=& \nabla_{\kappa} a(b+2) V_P^{b+1} + \nabla_{\rho_0} ab V_P^{b-1} \nonumber\\
                   &=& \left( \nabla_{\kappa} \frac{b+2}{b} V_P^2 + \nabla_{\rho_0} \right) ab V_P^{b-1} \nonumber
    \end{eqnarray}

  \end{minipage} \vline
  \begin{minipage}{0.45\linewidth}
    \[ V_P = \left(\frac{\kappa}{a}\right)^{\frac{1}{b+2}} \]
    
    \begin{eqnarray}
      \nabla_{\kappa} &=& \nabla_{V_P} \partderi{V_P}{\kappa} \nonumber\\
                      &=& \nabla_{V_P} \frac{1}{a(b+2)} \left(\frac{\kappa}{a}\right)^{-\frac{b+1}{b+2}} \nonumber
    \end{eqnarray}
  \end{minipage}

\end{frame}

\begin{frame}\frametitle{PARAMETERIZATION velocities-density}
\framesubtitle{isotropic P-SV}
  
  \begin{minipage}{0.5\linewidth}
    \[\left\{ \begin{array}{l}
      \lambda = \rho (V_P^2-2V_S^2) \\
      \mu    = \rho V_S^2 \\
      \rho_0 = \rho 
    \end{array} \right.\]
    
    \begin{eqnarray}
      \nabla_{V_P} &=& \nabla_\lambda \partderi{\lambda}{V_P} + \nabla_\mu \partderi{\mu}{V_P} + \nabla_{\rho_0} \partderi{\rho_0}{V_P} \nonumber\\
                   &=& \nabla_\lambda 2\rho V_P \nonumber\\
      \nabla_{V_S} &=& \nabla_\lambda \partderi{\lambda}{V_S} + \nabla_\mu \partderi{\mu}{V_S} + \nabla_{\rho_0} \partderi{\rho_0}{V_S} \nonumber\\
                   &=& \nabla_\lambda (-4)\rho V_S + \nabla_\mu 2\rho V_S \nonumber\\
                   &=& \left(-\nabla_\lambda 2 + \nabla_\mu \right) 2\rho V_S \nonumber\\
      \nabla_{\rho} &=& \nabla_\lambda \partderi{\lambda}{\rho} + \nabla_\mu \partderi{\mu}{\rho} + \nabla_{\rho_0} \partderi{\rho_0}{\rho} \nonumber\\
		    &=& \nabla_\lambda (V_P^2-2V_S^2) + \nabla_\mu V_S^2 + \nabla_{\rho_0} \nonumber
    \end{eqnarray}

  \end{minipage} \vline
  \begin{minipage}{0.45\linewidth}
    \[\left\{ \begin{array}{l}
      V_P  = \sqrt{\frac{\lambda+2\mu}{\rho_0}} \\
      V_S  = \sqrt{\frac{\mu}{\rho_0}} \\
      \rho = \rho_0
    \end{array} \right.\]
    
    \begin{eqnarray}
      \nabla_{\lambda}&=& \nabla_{V_P} \partderi{V_P}{\lambda} + \nabla_{V_S} \partderi{V_S}{\lambda} + \nabla_{\rho} \partderi{\rho}{\lambda} \nonumber\\
                      &=& ... \nonumber\\
      \nabla_{\mu}    &=& \nabla_{V_P} \partderi{V_P}{\mu}     + \nabla_{V_S} \partderi{V_S}{\mu}     + \nabla_{\rho} \partderi{\rho}{\mu} \nonumber\\
		      &=& ... \nonumber\\
      \nabla_{\rho_0} &=& \nabla_{V_P} \partderi{V_P}{\rho_0}  + \nabla_{V_S} \partderi{V_S}{\rho_0}  + \nabla_{\rho} \partderi{\rho}{\rho_0} \nonumber\\
		      &=& ... \nonumber
    \end{eqnarray}
  \end{minipage}

\end{frame}

\begin{frame}\frametitle{PARAMETERIZATION velocities-density  + PASSIVE gardner}
\framesubtitle{isotropic P-SV}

  \begin{center}
    \framebox{$\rho = a V_P ^{b}$}
  \end{center}
  
  \begin{minipage}{\linewidth}
    \[\left\{ \begin{array}{l}
      \lambda = \rho (V_P^2-2V_S^2) = a V_P^{b+2} - 2a V_P^{b} V_S^2 \\
      \mu    = \rho V_S^2 = a V_P ^{b}V_S^2 \\
      \rho_0 = \rho = a V_P ^{b}
    \end{array} \right.\]
    
    \begin{eqnarray}
      \nabla_{V_P} &=& \nabla_\lambda \partderi{\lambda}{V_P} + \nabla_\mu \partderi{\mu}{V_P} + \nabla_{\rho_0} \partderi{\rho_0}{V_P} \nonumber\\
                   &=& \nabla_\lambda \left( a(b+2)V_P^{b+1} - 2abV_P^{b-1}V_S^2\right) + \nabla_\mu     abV_P^{b-1}V_S^2 + \nabla_{\rho_0} abV_P^{b-1} \nonumber\\
                   &=& \left( \nabla_\lambda \left( \frac{b+2}{b}V_P^2 - 2V_S^2 \right) + \nabla_\mu V_S^2 + \nabla_{\rho_0} \right)abV_P^{b-1} \nonumber\\
      \nabla_{V_S} &=& \nabla_\lambda \partderi{\lambda}{V_S} + \nabla_\mu \partderi{\mu}{V_S} + \nabla_{\rho_0} \partderi{\rho_0}{V_S} \nonumber\\
                   &=& \nabla_\lambda (-4a V_P^{b}V_S) + \nabla_\mu 2aV_P^{b}V_S \nonumber\\
                   &=& \left(\nabla_\lambda (-2) + \nabla_\mu \right)2aV_P^{b}V_S \nonumber
    \end{eqnarray}

  \end{minipage}
  
\end{frame}


\section{velocities-impedance}

\begin{frame}\frametitle{PARAMETERIZATION velocities-impedance}
\framesubtitle{isotropic ACoustic}

  \begin{center}
    \framebox{$I_P = V_P \rho$}
  \end{center}
  
  \begin{minipage}{0.45\linewidth}
    \[\left\{ \begin{array}{l}
      \kappa = \rho V_P^2 = V_PI_P \\
      \rho_0 = \rho = \frac{I_P}{V_P}
    \end{array} \right.\]
    
    \begin{eqnarray}
      \nabla_{V_P} &=& \nabla_{\kappa} \partderi{\kappa}{V_P} + \nabla_{\rho_0} \partderi{\rho_0}{V_P} \nonumber\\
                   &=& \nabla_{\kappa} I_P + \nabla_{\rho_0} (-I_PV_P^{-2}) \nonumber\\
      \nabla_{I_P} &=& \nabla_{\kappa} \partderi{\kappa}{I_P} + \nabla_{\rho_0} \partderi{\rho_0}{I_P} \nonumber\\
		   &=& \nabla_{\kappa} V_P + \nabla_{\rho_0} V_P^{-1} \nonumber
    \end{eqnarray}

  \end{minipage} \vline
  \begin{minipage}{0.45\linewidth}
    \[\left\{ \begin{array}{l}
      V_P  = \sqrt{\frac{\kappa}{\rho_0}} \\
      I_P = \sqrt{\kappa\rho_0}
    \end{array} \right.\]
    
    \begin{eqnarray}
      \nabla_{\kappa} &=& \nabla_{V_P} \partderi{V_P}{\kappa} + \nabla_{I_P} \partderi{I_P}{\kappa} \nonumber\\
                      &=& \nabla_{V_P} \frac{1}{2\rho_0}\sqrt{\frac{\rho_0}{\kappa}} + \nabla_{I_P} \frac{\rho_0}{2\sqrt{\kappa\rho_0}} \nonumber\\
                      &=& \nabla_{V_P} 0.5\rho_0^{-0.5}\kappa^{-0.5} + \nabla_{I_P} 0.5\rho_0^{0.5}\kappa^{-0.5} \nonumber\\
                      &=& \left( \nabla_{V_P} + \nabla_{I_P} \rho_0 \right) 0.5\rho_0^{-0.5}\kappa^{-0.5} \nonumber\\
      \nabla_{\rho_0} &=& \nabla_{V_P} \partderi{V_P}{\rho_0} + \nabla_{I_P} \partderi{I_P}{\rho_0} \nonumber\\
                      &=& \nabla_{V_P} \frac{-\kappa}{2\rho_0^2}\sqrt{\frac{\rho_0}{\kappa}} + \nabla_{I_P} \frac{\kappa}{2\sqrt{\kappa\rho_0}} \nonumber\\
                      &=& \nabla_{V_P} (-0.5)\rho_0^{-1.5}\kappa^{0.5} + \nabla_{I_P} 0.5\rho_0^{-0.5}\kappa^{0.5} \nonumber\\
                      &=& \left(-\nabla_{V_P}\rho_0^{-1} + \nabla_{I_P} \right) 0.5\rho_0^{-0.5}\kappa^{0.5} \nonumber
    \end{eqnarray}
  \end{minipage}

\end{frame}

\begin{frame}\frametitle{PARAMETERIZATION velocities-impedance}
\framesubtitle{isotropic P-SV}

%   \begin{center}
%     \framebox{$I_P = V_P \rho$}
%   \end{center}
  
  \begin{minipage}{\linewidth}
    \[\left\{ \begin{array}{l}
      \lambda = \rho (V_P^2-2V_S^2) = V_PI_P - \frac{2V_S^2I_P}{V_P} \\
      \mu    = \rho V_S^2 = \frac{V_S^2I_P}{V_P} \\
      \rho_0 = \rho = \frac{I_P}{V_P}
    \end{array} \right.\]
    
    \begin{eqnarray}
      \nabla_{V_P} &=& \nabla_\lambda \partderi{\lambda}{V_P} + \nabla_\mu \partderi{\mu}{V_P} + \nabla_{\rho_0} \partderi{\rho_0}{V_P} \nonumber\\
                   &=& \nabla_\lambda \left(I_P+\frac{2V_S^2I_P}{V_P^2}\right) + \nabla_\mu \left(-\frac{V_S^2I_P}{V_P^2}\right) + \nabla_{\rho_0} \left(-\frac{I_P}{V_P^2}\right) \nonumber\\
                   &=& \nabla_\lambda \left(I_P+\frac{2V_S^2I_P}{V_P^2}\right) + \nabla_\mu \left(-\frac{V_S^2I_P}{V_P^2}\right) + \nabla_{\rho_0} \left(-\frac{I_P}{V_P^2}\right) \nonumber\\
                   &=& \left( \nabla_\lambda (V_P^2+2V_S^2) - \nabla_\mu V_S^2 - \nabla_{\rho_0} \right) \frac{I_P}{V_P^2} \nonumber\\
      \nabla_{V_S} &=& \nabla_\lambda \partderi{\lambda}{V_S} + \nabla_\mu \partderi{\mu}{V_S} + \nabla_{\rho_0} \partderi{\rho_0}{V_S} \nonumber\\
                   &=& \nabla_\lambda \frac{-4V_SI_P}{V_P} + \nabla_\mu \frac{2V_SI_P}{V_P} \nonumber\\
                   &=& \left( -2\nabla_\lambda + \nabla_\mu \right) \frac{2V_SI_P}{V_P} \nonumber
    \end{eqnarray}

  \end{minipage} %\vline
%   \begin{minipage}{0.45\linewidth}
%     \[\left\{ \begin{array}{l}
%       V_P  = \sqrt{\frac{\lambda+2\mu}{\rho_0}} \\
%       V_S  = \sqrt{\frac{\mu}{\rho_0}} \\
%       \rho = \rho_0
%     \end{array} \right.\]
%     
%     \begin{eqnarray}
%       \nabla_{\lambda}&=& \nabla_{V_P} \partderi{V_P}{\lambda} + \nabla_{V_S} \partderi{V_S}{\lambda} + \nabla_{\rho} \partderi{\rho}{\lambda} \nonumber\\
%                       &=& ... \nonumber\\
%       \nabla_{\mu}    &=& \nabla_{V_P} \partderi{V_P}{\mu}     + \nabla_{V_S} \partderi{V_S}{\mu}     + \nabla_{\rho} \partderi{\rho}{\mu} \nonumber\\
% 		      &=& ... \nonumber\\
%       \nabla_{\rho_0} &=& \nabla_{V_P} \partderi{V_P}{\rho_0}  + \nabla_{V_S} \partderi{V_S}{\rho_0}  + \nabla_{\rho} \partderi{\rho}{\rho_0} \nonumber\\
% 		      &=& ... \nonumber
%     \end{eqnarray}
%   \end{minipage}

\end{frame}

\begin{frame}\frametitle{PARAMETERIZATION velocities-impedance}
\framesubtitle{isotropic P-SV \textit{continued}}
  \begin{minipage}{\linewidth}
    \[\left\{ \begin{array}{l}
      \lambda = \rho (V_P^2-2V_S^2) = V_PI_P - \frac{2V_S^2I_P}{V_P} \\
      \mu    = \rho V_S^2 = \frac{V_S^2I_P}{V_P} \\
      \rho_0 = \rho = \frac{I_P}{V_P}
    \end{array} \right.\]
    
    \begin{eqnarray}
      \nabla_{I_P} &=& \nabla_\lambda \partderi{\lambda}{I_P} + \nabla_\mu \partderi{\mu}{I_P} + \nabla_{\rho_0} \partderi{\rho_0}{I_P} \nonumber\\
		   &=& \nabla_\lambda \left(V_P-\frac{2V_S^2}{V_P}\right) + \nabla_\mu \frac{V_S^2}{V_P} + \nabla_{\rho_0} \frac{1}{V_P} \nonumber\\
		   &=& \left( \nabla_\lambda (V_P^2-2V_S^2) + \nabla_\mu V_S^2 + \nabla_{\rho_0} \right) \frac{1}{V_P} \nonumber
    \end{eqnarray}
  \end{minipage}
\end{frame}

\section{slowness-density}

\begin{frame}\frametitle{PARAMETERIZATION slowness-density}
\framesubtitle{isotropic ACoustic}

  \begin{center}
    \framebox{$S_P = 1/V_P$}
  \end{center}
  
  \begin{minipage}{0.5\linewidth}
    \[\left\{ \begin{array}{l}
      \kappa = \rho V_P^2 = \rho S_P^{-2} \\
      \rho_0 = \rho 
    \end{array} \right.\]
    
    \begin{eqnarray}
      \nabla_{S_P} &=& \nabla_{\kappa} \partderi{\kappa}{S_P} + \nabla_{\rho_0} \partderi{\rho_0}{S_P} \nonumber\\
                   &=& \nabla_{\kappa} (-2\rho S_P^{-3})  \nonumber\\
      \nabla_{\rho} &=& \nabla_{\kappa} \partderi{\kappa}{\rho} + \nabla_{\rho_0} \partderi{\rho_0}{\rho} \nonumber\\
		    &=& \nabla_{\kappa} S_P^{-2} + \nabla_{\rho_0} \nonumber
    \end{eqnarray}

  \end{minipage} \vline
  \begin{minipage}{0.45\linewidth}
    \[\left\{ \begin{array}{l}
      S_P  = \sqrt{\frac{\rho_0}{\kappa}} \\
      \rho = \rho_0
    \end{array} \right.\]
    
    \begin{eqnarray}
      \nabla_{\kappa} &=& \nabla_{S_P} \partderi{S_P}{\kappa} + \nabla_{\rho} \partderi{\rho}{\kappa} \nonumber\\
                      &=& \nabla_{S_P} \left(\frac{1}{2}\sqrt{\frac{\kappa}{\rho_0}}\frac{-\rho_0}{\kappa^2}\right) \nonumber\\
                      &=& \nabla_{S_P} (-0.5)\rho_0^{0.5}\kappa^{-1.5} \nonumber\\
      \nabla_{\rho_0} &=& \nabla_{S_P} \partderi{S_P}{\rho_0} + \nabla_{\rho} \partderi{\rho}{\rho_0} \nonumber\\
                      &=& \nabla_{S_P} \left(\frac{1}{2}\sqrt{\frac{\kappa}{\rho_0}}\frac{1}{\kappa}\right) + \nabla_{\rho} \nonumber\\
                      &=& \nabla_{S_P} 0.5\rho_0^{-0.5}\kappa^{-0.5} + \nabla_{\rho} \nonumber
    \end{eqnarray}
  \end{minipage}

\end{frame}

\begin{frame}\frametitle{PARAMETERIZATION slowness-density + PASSIVE gardner}
\framesubtitle{isotropic ACoustic}

  \begin{center}
    \framebox{$\rho = a S_P^{-b}$}
  \end{center}

  \begin{minipage}{0.5\linewidth}
    \[\left\{ \begin{array}{l}
      \kappa = \rho V_P^2 = a S_P^{-b-2} \\
      \rho_0 = \rho = a S_P ^{-b}
    \end{array} \right.\]
    
    \begin{eqnarray}
      \nabla_{S_P} &=& \nabla_{\kappa} \partderi{\kappa}{S_P} + \nabla_{\rho_0} \partderi{\rho_0}{S_P} \nonumber\\
                   &=& \nabla_{\kappa} a(-b-2) S_P^{-b-3} \nonumber\\
                   & &+\nabla_{\rho_0} (-ab) S_P^{-b-1} \nonumber\\
                   &=&-\left( \nabla_{\kappa} a(b+2) + \nabla_{\rho_0} abS_P^2 \right) S_P^{-b-3} \nonumber
    \end{eqnarray}

  \end{minipage} \vline
  \begin{minipage}{0.45\linewidth}
    \[ S_P = \left(\frac{\kappa}{a}\right)^{-\frac{1}{b+2}} \]
    
    \begin{eqnarray}
      \nabla_{\kappa} &=& \nabla_{S_P} \partderi{S_P}{\kappa} \nonumber\\
                      &=& \nabla_{S_P} \frac{-1}{a(b+2)} \left(\frac{\kappa}{a}\right)^{-\frac{b+3}{b+2}} \nonumber
    \end{eqnarray}
  \end{minipage}

\end{frame}


\begin{frame}\frametitle{PARAMETERIZATION slowness-density}
\framesubtitle{isotropic P-SV}
  
  \begin{center}
    \framebox{$S_{PS} = V_S/V_P = V_SS_P$}
  \end{center}
  
  \[\left\{ \begin{array}{l}
    \lambda = \rho (V_P^{2}-2V_S ^2) = \rho S_P^{-2} (1-2S_{PS}^2) \\
    \mu    = \rho V_S^2 = \rho (S_{PS}/S_P)^2 \\
    \rho_0 = \rho 
  \end{array} \right.\]
  
  \begin{eqnarray}
    \nabla_{S_P} &=& \nabla_\lambda \partderi{\lambda}{S_P} + \nabla_\mu \partderi{\mu}{S_P} + \nabla_{\rho_0} \partderi{\rho_0}{S_P} \nonumber\\
		 &=& \nabla_\lambda \rho(-2)S_P^{-3}(1-2S_{PS}^2) + \nabla_\mu \rho S_{PS}^2(-2)S_P^{-3} \nonumber\\
		 &=& \left(\nabla_\lambda (1-2S_{PS}^2) + \nabla_\mu S_{PS}^2 \right)(-2)\rho S_P^{-3} \nonumber\\
    \nabla_{S_{PS}} &=& \nabla_\lambda \partderi{\lambda}{S_{PS}} + \nabla_\mu \partderi{\mu}{S_{PS}} + \nabla_{\rho_0} \partderi{\rho_0}{S_{PS}} \nonumber\\
		    &=& \nabla_\lambda \rho S_P^{-2}(-4)S_{PS} + \nabla_\mu 2\rho S_{PS}/S_P^2 \nonumber\\
		    &=& \left(-\nabla_\lambda 2 + \nabla_\mu \right) 2\rho S_{PS} S_P^{-2} \nonumber\\
    \nabla_{\rho} &=& \nabla_\lambda \partderi{\lambda}{\rho} + \nabla_\mu \partderi{\mu}{\rho} + \nabla_{\rho_0} \partderi{\rho_0}{\rho} \nonumber\\
		  &=& \nabla_\lambda S_P^{-2} (1-2S_{PS}^2) + \nabla_\mu (S_{PS}/S_P)^2 + \nabla_{\rho_0} \nonumber\\
		  &=& \left(\nabla_\lambda (1-2S_{PS}^2) + \nabla_\mu S_{PS} \right) S_P^{-2} + \nabla_{\rho_0} \nonumber
  \end{eqnarray}

\end{frame}

\begin{frame}\frametitle{PARAMETERIZATION slowness-density  + PASSIVE gardner}
\framesubtitle{isotropic P-SV}

  \begin{center}
    \framebox{$S_{PS} = V_SS_P; \rho = a S_P^{-b}$}
  \end{center}
  
  \[\left\{ \begin{array}{l}
    \lambda = \rho S_P^{-2} (1-2S_{PS}^2) = a S_P^{-b-2} (1-2S_{PS}^2) \\
    \mu    = \rho (S_{PS}/S_P)^2 = a S_P^{-b-2} S_{PS}^2\\
    \rho_0 = a S_P^{-b}
  \end{array} \right.\]
  
  \begin{eqnarray}
    \nabla_{S_P} &=& \nabla_\lambda \partderi{\lambda}{S_P} + \nabla_\mu \partderi{\mu}{S_P} + \nabla_{\rho_0} \partderi{\rho_0}{S_P} \nonumber\\
		 &=& \nabla_\lambda a(-b-2)S_P^{-b-3}(1-2S_{PS}^2) \nonumber\\
		 & &+\nabla_\mu a(-b-2) S_P^{-b-3}S_{PS}^2 + \nabla_{\rho_0} a(-b)S_P^{-b-1} \nonumber\\
		 &=& \left(\nabla_\lambda (b+2)(1-2S_{PS}^2) + \nabla_\mu (b+2)S_{PS}^2 + \nabla_{\rho_0} bS_P^2 \right) (-a) S_P^{-b-3} \nonumber\\
    \nabla_{S_{PS}} &=& \nabla_\lambda \partderi{\lambda}{S_{PS}} + \nabla_\mu \partderi{\mu}{S_{PS}} + \nabla_{\rho_0} \partderi{\rho_0}{S_{PS}} \nonumber\\
		    &=& \nabla_\lambda a S_P^{-b-2} (-4)S_{PS} + \nabla_\mu a S_P^{-b-2} 2S_{PS} \nonumber\\
		    &=& \left(-\nabla_\lambda 2 + \nabla_\mu \right) 2aS_P^{-b-2}S_{PS}\nonumber\\
  \end{eqnarray}

\end{frame}

\end{document}



%%%%%%%%%%%%%%%%%%%%%%%%%%%%
%%%%%% GOOD THINGS %%%%%%%%%
% %-------------------------------------------------------------------------------------
% \frame{
%  %\MyLogo
% \frametitle{}
% 
% \vspace*{\fill} 
% \begin{minipage}[c][8cm]{5cm}
% \begin{itemize}
% \item Source in red
% \item Receiver in blue
% \end{itemize}
% \end{minipage}
% 
% \begin{block}{Algorithm}
% %\footnotesize{
% \begin{algorithmic}[1]
% %%-----------------------------------------------
% \FOR {$frequency = frequency\_1$ to $frequency\_n$}
% \WHILE {(NOT $convergence$ AND $iter<niter_{max}$)}
% \STATE Estimate source wavelet if required
% \STATE Build gradient vector ${\mathcal{G}}_{\bf{m}}^{(k)}$
% \STATE Build perturbation vector $\delta \bf{m}$
% \STATE Update model ${\bf{m}}^{(k+1)} = {\bf{m}}^{(k)} + \alpha  \delta {\bf{m}}$
% \ENDWHILE
% \ENDFOR
% %%-----------------------------------------------
% \label{algo1}
% \end{algorithmic}
% %\end{algorithm}
% %}
% \end{block}
% }
%
% \colorbox{yellow}{reflection data}
%
% % Fontsize
%     \tiny
%     \scriptsize
%     \footnotesize
%     \small
%     \normalsize
%     \large
%     \Large
%     \LARGE
%     \huge
%     \Huge 
%
% % Multiple equations 
% \begin{eqnarray}
% \delta C & = &  p \\
%          & = &  p \rangle
% \label{eq}
% \end{eqnarray}
%add multiple eq. indices
%
% \[ f(n) = \left\{
%   \begin{array}{l l}
%          n/2 & \quad \text{if $n$ is even}\\
%     -(n+1)/2 & \quad \text{if $n$ is odd}
%   \end{array} \right.\]
%can't use {equation} because it's an array (can't add eq. index)
%
%\begin{equation}
%  u(x) =
%   \begin{cases}
%    \exp{x} & \text{if } x \geq 0 \\
%    1       & \text{if } x < 0
%   \end{cases}
%\end{equation}
%can use {equation} because it's an equation (can add eq. index)
%
% % Split an equation into multiple lines
%   \begin{equation}
%   \begin{split}
%     f(x) & =  1 \\
% 	  & -  g(x)
%   \end{split}
%   \end{equation}
% %-------------------------------------------------------------------------------------
%%%%%%%%%%%%%%%%%%%%%%%%%%%%


